Fixes for tight equality

examples/temporal_deep/src/examples/ltl2omega.sml
@@ -1,62 +1,32 @@
-(*
-quietdec := true;
+open HolKernel boolLib bossLib;
 
-val home_dir = (concat Globals.HOLDIR "/examples/temporal_deep/");
-loadPath := (concat home_dir "src/deep_embeddings") ::
-            (concat home_dir "src/translations") ::
-            (concat home_dir "src/tools") ::
-            (concat hol_dir "examples/PSL/path") ::
-            (concat hol_dir "examples/PSL/1.1/official-semantics") :: !loadPath;
-
-map load
- ["full_ltlTheory", "arithmeticTheory", "automaton_formulaTheory", "xprop_logicTheory", "prop_logicTheory",
-  "infinite_pathTheory", "tuerk_tacticsLib", "symbolic_semi_automatonTheory", "listTheory", "pred_setTheory",
-  "temporal_deep_mixedTheory", "pred_setTheory", "rich_listTheory", "set_lemmataTheory", "pairTheory",
-  "ltl_to_automaton_formulaTheory",
-  "numLib", "listLib", "translationsLib", "rltlTheory",
-  "rltl_to_ltlTheory", "psl_to_rltlTheory", "UnclockedSemanticsTheory",
-  "SyntacticSugarTheory", "congLib", "temporal_deep_simplificationsLib"];
-*)
-
-open HolKernel boolLib bossLib  full_ltlTheory arithmeticTheory automaton_formulaTheory xprop_logicTheory prop_logicTheory
+open full_ltlTheory arithmeticTheory automaton_formulaTheory xprop_logicTheory prop_logicTheory
      infinite_pathTheory tuerk_tacticsLib symbolic_semi_automatonTheory listTheory pred_setTheory
      temporal_deep_mixedTheory pred_setTheory rich_listTheory set_lemmataTheory pairTheory rltlTheory
-     ltl_to_automaton_formulaTheory numLib listLib translationsLib rltl_to_ltlTheory psl_to_rltlTheory UnclockedSemanticsTheory
+     ltl_to_automaton_formulaTheory numLib listLib translationsLib
+     rltl_to_ltlTheory psl_to_rltlTheory UnclockedSemanticsTheory
      SyntacticSugarTheory congLib temporal_deep_simplificationsLib;
-
-
-(*
-show_assums := false;
-show_assums := true;
-show_types := true;
-show_types := false;
-quietdec := false;
-*)
-
 
 (* A function to generate test ltl formulas.
    This has been kindly provided by Kristin Yvonne Rozier <kyrozier@cs.rice.edu>
 
    Input: n = the number of bits in the counter
-   Output: an LTL formula describing an n-bit counter*)
-
+   Output: an LTL formula describing an n-bit counter
+ *)
 local
 
-  fun  mpattern_int 0 = ``LTL_NEXT (m:'a ltl)``
+  fun mpattern_int 0 = ``LTL_NEXT (m:'a ltl)``
     | mpattern_int n = subst [mk_var ("X", ``:'a ltl``) |-> mpattern_int (n-1)]
                           ``LTL_NEXT (LTL_AND(LTL_NOT (m:'a ltl), X))``;
 
   fun mpattern n = subst [mk_var ("X", ``:'a ltl``) |-> mpattern_int n]
                         ``LTL_AND((m:'a ltl), LTL_ALWAYS (LTL_IMPL (m, X)))``;
 
-
-
-  fun  bpattern 0 = ``LTL_NOT (b:'a ltl)``
+  fun bpattern 0 = ``LTL_NOT (b:'a ltl)``
     | bpattern n = subst [mk_var ("X", ``:'a ltl``) |-> bpattern (n-1)]
                         ``LTL_AND(LTL_NOT (b:'a ltl), LTL_NEXT X)`` ;
 
-
-  fun  nest_next_pattern 0 t = t
+  fun nest_next_pattern 0 t = t
     | nest_next_pattern n t = liteLib.mk_icomb (``LTL_NEXT:'a ltl->'a ltl``, nest_next_pattern (n-1) t)
 
   fun nest_pattern n =
@@ -111,14 +81,8 @@ in
 
 end;
 
-
-
-
-
-
-
 val pslTerm = ``
-F_ALWAYS (F_IMPLIES(F_STRONG_BOOL (B_PROP aa),
+    F_ALWAYS (F_IMPLIES(F_STRONG_BOOL (B_PROP aa),
                     F_STRONG_NEXT_EVENT (B_PROP bb,
                                          F_STRONG_BEFORE (
                                             F_STRONG_BOOL (B_PROP cc),
@@ -146,19 +110,12 @@ val ltlTermSimp = rand ( concl (
    Simulation Relations for Alternating Buechi Automata" by Carsten Fritz*)
 
 val test0LTL = ``
-LTL_NOT (LTL_SUNTIL (
-    LTL_SUNTIL(LTL_NEXT (LTL_PROP (P_PROP  b)), LTL_NOT(LTL_SUNTIL (LTL_NOT (LTL_ALWAYS (LTL_PROP (P_PROP  a))), LTL_NOT (LTL_PROP (P_PROP  c))))),
-
-    LTL_NOT(
-        LTL_SUNTIL (
-            LTL_NOT (LTL_ALWAYS (LTL_NOT (LTL_PROP (P_PROP  a)))),
-            LTL_NOT (LTL_PROP (P_PROP  a))
-        )
-    )
-))``;
-
-
-
+    LTL_NOT
+     (LTL_SUNTIL (LTL_SUNTIL (LTL_NEXT (LTL_PROP (P_PROP b)),
+                              LTL_NOT (LTL_SUNTIL (LTL_NOT (LTL_ALWAYS (LTL_PROP (P_PROP a))),
+                                                   LTL_NOT (LTL_PROP (P_PROP  c))))),
+                  LTL_NOT (LTL_SUNTIL (LTL_NOT (LTL_ALWAYS (LTL_NOT (LTL_PROP (P_PROP a)))),
+                                       LTL_NOT (LTL_PROP (P_PROP a))))))``;
 
 val test1LTL = ``LTL_PROP (P_PROP a)``;
 val test2LTL = ``LTL_NOT(LTL_PROP (P_PROP a))``;
@@ -189,16 +146,18 @@ LTL_OR(
         LTL_PROP (P_PROP e)),
       LTL_PSUNTIL
         (LTL_NOT (LTL_SUNTIL (LTL_PROP P_TRUE,LTL_NOT (LTL_PROP (P_PROP d)))),
-        LTL_PROP (P_PROP b))))``
+        LTL_PROP (P_PROP b))))``;
+
 val test14LTL = ``LTL_EQUIV(LTL_NOT(LTL_PROP (P_PROP a)), LTL_PROP (P_PROP b))``;
 
-
+(* p U q *)
+val test15LTL = ``LTL_SUNTIL (LTL_PROP (P_PROP p), LTL_PROP (P_PROP q))``;
 
 val test1RLTL = ``RLTL_PROP (P_PROP a)``;
 val test2RLTL = ``RLTL_NOT(RLTL_PROP (P_PROP (a:'c)))``;
-val test3RLTL = ``RLTL_ACCEPT(RLTL_SUNTIL (RLTL_PROP (P_PROP a),
-RLTL_NEXT(RLTL_PROP (P_PROP a))), P_PROP c)``;
-
+val test3RLTL = ``RLTL_ACCEPT (RLTL_SUNTIL (RLTL_PROP (P_PROP a),
+                                            RLTL_NEXT (RLTL_PROP (P_PROP a))),
+                               P_PROP c)``;
 
 (*Some examples to execute at interactivly. Just change the
   number of the test terms or introduce on terms *)
@@ -206,7 +165,16 @@ RLTL_NEXT(RLTL_PROP (P_PROP a))), P_PROP c)``;
 (*
 
 ltl2omega false false test13LTL
-ltl2omega true false test13LTL
+ltl2omega true  false test13LTL
+
+(* syntax: ltl2omega fast neg ltl *)
+
+ltl2omega false (* no-fast *) false (* orig *) test15LTL;
+ltl2omega false (* no-fast *) true  (* neg *)  test15LTL;
+ltl2omega true false test15LTL;
+ltl2omega true true test15LTL;
+ltl2omega_rewrite true  (* max *) test15LTL; (* p U q *)
+ltl2omega_rewrite false (* min *) test15LTL; (* p U q *)
 
 ************************************************
 The fast switch has some influence. Notice the
@@ -234,7 +202,6 @@ just rewriting. Just a proof of concept
 ************************************************
 time (ltl2omega_rewrite true) test11LTL
 
-
 ************************************************
 Translations to kripke_structure
 ************************************************
@@ -244,19 +211,14 @@ time (ltl_contradiction2ks_fair_emptyness___num 1 true) test11LTL
 time (ltl_contradiction2ks_fair_emptyness___num 2 true) test11LTL
 time (ltl_contradiction2ks_fair_emptyness___num 3 true) test11LTL
 
-
 time (ltl_contradiction2ks_fair_emptyness true) test13LTL
 time (ltl_contradiction2ks_fair_emptyness___num 1 true) test13LTL
 time (ltl_contradiction2ks_fair_emptyness___num 2 true) test13LTL
 time (ltl_contradiction2ks_fair_emptyness___num 3 true) test13LTL
 
-
-
-val ltl_ks_sem2ks_fair_emptyness___no_ks : bool -> Abbrev.term -> Abbrev.thm
-val ltl_ks_sem2ks_fair_emptyness : bool -> Abbrev.term -> Abbrev.term -> Abbrev.thm
-
-  val ltl_equivalent2ks_fair_emptyness : bool -> Abbrev.term -> Abbrev.term -> Abbrev.thm
-
+val ltl_ks_sem2ks_fair_emptyness___no_ks : bool -> term -> thm
+val ltl_ks_sem2ks_fair_emptyness : bool -> term -> term -> thm
+val ltl_equivalent2ks_fair_emptyness : bool -> term -> term -> thm
 
 *************************************************
 LTL counters
@@ -267,7 +229,6 @@ using the "slow" version
 *************************************************
 time (ltl2omega false true) (ltl_counter 2)
 time (ltl2omega true true) (ltl_counter 2)
-
 
 ************************************************
 You may also be interested in the following
@@ -287,5 +248,3 @@ LTL_TO_GEN_BUECHI_DS___MIN_FAIR_RUN_def
 LTL_TO_GEN_BUECHI_DS___MAX_FAIR_RUN_def
 
 *)
-
-
